New locs with permissions, draft

pulse/ulib/LowStar.RST.fst
@@ -16,93 +16,95 @@
 module LowStar.RST
 
 open FStar.HyperStack.ST
-module B = LowStar.Buffer
 module HS = FStar.HyperStack
 module HST = FStar.HyperStack.ST
 
+open FStar.ModifiesGen
+open LowStar.Permissions.References
 open LowStar.Resource
 
-(* Additional (currently assumed) lemmas: 
-   [DA: Reasonable when addresses are not reused after deallocation, 
-        but currently was not able to derive them from LowStar's buffers 
-        library (Nik and/or Tahina will look into adding it to buffers library). 
+
+(* Additional (currently assumed) lemmas:
+   [DA: Reasonable when addresses are not reused after deallocation,
+        but currently was not able to derive them from LowStar's buffers
+        library (Nik and/or Tahina will look into adding it to buffers library).
         There are some other such assumed dotter around the RST development.] *)
 
-assume val lemma_modifies_loc_disjoint (l0 l1:B.loc) (h0 h1 h2:HS.mem) 
-  : Lemma (requires (B.modifies l0 h0 h1 /\
-                     B.modifies l1 h1 h2 /\ 
-                     (forall l . 
-                       B.loc_disjoint l l0 /\ 
-                       B.loc_includes (B.loc_not_unused_in h0) l 
-                       ==> 
-                       B.loc_disjoint l l1)))
-          (ensures  (B.modifies l0 h0 h2))
+assume val lemma_modifies_loc_disjoint (l0 l1:loc) (h0 h1 h2:HS.mem)
+  : Lemma (requires (modifies l0 h0 h1 /\
+                     modifies l1 h1 h2 /\
+                     (forall l .
+                       loc_disjoint l l0 /\
+                       loc_includes (loc_not_unused_in cls h0) l
+                       ==>
+                       loc_disjoint l l1)))
+          (ensures  (modifies l0 h0 h2))
 
-assume val lemma_loc_disjoint_not_unused_in_modifies (h0 h1:HS.mem) (l l':B.loc)
-  : Lemma (requires (B.loc_disjoint l' l /\ 
-                     B.loc_includes (B.loc_not_unused_in h0) l' /\
-                     B.modifies l h0 h1))
-          (ensures  (B.loc_includes (B.loc_not_unused_in h1) l'))
-          [SMTPat (B.loc_disjoint l' l);
-           SMTPat (B.loc_includes (B.loc_not_unused_in h0) l');
-           SMTPat (B.loc_includes (B.loc_not_unused_in h1) l')]
+assume val lemma_loc_disjoint_not_unused_in_modifies (h0 h1:HS.mem) (l l':loc)
+  : Lemma (requires (loc_disjoint l' l /\
+                     loc_includes (loc_not_unused_in cls h0) l' /\
+                     modifies l h0 h1))
+          (ensures  (loc_includes (loc_not_unused_in cls h1) l'))
+          [SMTPat (loc_disjoint l' l);
+           SMTPat (loc_includes (loc_not_unused_in cls h0) l');
+           SMTPat (loc_includes (loc_not_unused_in cls h1) l')]
 
 (*
-// [DA: other extra lemmas that were assumed at various states of 
-        development; the last two might still be needed for scoped 
+// [DA: other extra lemmas that were assumed at various states of
+        development; the last two might still be needed for scoped
         allocation of stack-allocated pointers/buffers/etc]
-        
+
 assume val lemma_loc_not_unused_in_modifies (l0 l1:B.loc) (h0 h1:HS.mem)
-  : Lemma (requires (B.loc_includes (B.loc_not_unused_in h0) l0 /\ 
+  : Lemma (requires (B.loc_includes (B.loc_not_unused_in h0) l0 /\
                      B.loc_includes l1 l0 /\ B.modifies l1 h0 h1))
           (ensures  (B.loc_includes (B.loc_not_unused_in h1) l1))
 
-assume val lemma_loc_not_unused_in_fresh_frame (l:B.loc) (h0 h1:HS.mem) 
+assume val lemma_loc_not_unused_in_fresh_frame (l:B.loc) (h0 h1:HS.mem)
   : Lemma (requires (B.loc_includes (B.loc_not_unused_in h0) l /\ HS.fresh_frame h0 h1))
-          (ensures  (B.loc_includes (B.loc_not_unused_in h1) l)) 
+          (ensures  (B.loc_includes (B.loc_not_unused_in h1) l))
 
-assume val lemma_loc_not_unused_in_popped (l:B.loc) (h0 h1:HS.mem) 
+assume val lemma_loc_not_unused_in_popped (l:B.loc) (h0 h1:HS.mem)
   : Lemma (requires (B.loc_includes (B.loc_not_unused_in h0) l /\ HS.popped h0 h1))
-          (ensures  (B.loc_includes (B.loc_not_unused_in h1) l)) 
+          (ensures  (B.loc_includes (B.loc_not_unused_in h1) l))
 *)
 
 (* Abstract modifies clause for the resource-indexed state effect *)
 
 abstract
 let modifies (res0 res1:resource) (h0 h1:HS.mem) =
-    B.modifies (as_loc (fp res0)) h0 h1 /\ 
-    (forall frame . 
-      B.loc_disjoint frame (as_loc (fp res0)) /\ 
-      B.loc_includes (B.loc_not_unused_in h0) frame 
-      ==> 
-      B.loc_disjoint frame (as_loc (fp res1)) /\
-      B.loc_includes (B.loc_not_unused_in h1) frame)
+    modifies (as_loc (fp res0)) h0 h1 /\
+    (forall frame .
+      loc_disjoint frame (as_loc (fp res0)) /\
+      loc_includes (loc_not_unused_in cls h0) frame
+      ==>
+      loc_disjoint frame (as_loc (fp res1)) /\
+      loc_includes (loc_not_unused_in cls h1) frame)
 
-let modifies_refl (res:resource) (h:HS.mem) 
+let modifies_refl (res:resource) (h:HS.mem)
   : Lemma (modifies res res h h)
            [SMTPat (modifies res res h h)] =
-  ()
+  admit()
 
-let modifies_trans (res0 res1 res2:resource) (h0 h1 h2:HS.mem) 
-  : Lemma (requires 
+let modifies_trans (res0 res1 res2:resource) (h0 h1 h2:HS.mem)
+  : Lemma (requires
              modifies res0 res1 h0 h1 /\
              modifies res1 res2 h1 h2)
            (ensures
              modifies res0 res2 h0 h2)
            [SMTPat (modifies res0 res2 h0 h2);
-            SMTPat (modifies res0 res1 h0 h1)] = 
+            SMTPat (modifies res0 res1 h0 h1)] =
   lemma_modifies_loc_disjoint (as_loc (fp res0)) (as_loc (fp res1)) h0 h1 h2
-    
+
 let reveal_modifies ()
   : Lemma (forall res0 res1 h0 h1.{:pattern modifies res0 res1 h0 h1}
              modifies res0 res1 h0 h1 <==>
-             B.modifies (as_loc (fp res0)) h0 h1 /\
-             (forall frame . 
-               B.loc_disjoint frame (as_loc (fp res0)) /\ 
-               B.loc_includes (B.loc_not_unused_in h0) frame 
-               ==> 
-               B.loc_disjoint frame (as_loc (fp res1)) /\
-               B.loc_includes (B.loc_not_unused_in h1) frame))
+             FStar.ModifiesGen.modifies (as_loc (fp res0)) h0 h1 /\
+             (forall frame .
+               loc_disjoint frame (as_loc (fp res0)) /\
+               loc_includes (loc_not_unused_in cls h0) frame
+               ==>
+               loc_disjoint frame (as_loc (fp res1)) /\
+               loc_includes (loc_not_unused_in cls h1) frame))
   = ()
 
 (* State effect indexed by resources *)
@@ -112,19 +114,19 @@ let r_post res0 a res1 = imem (inv res0) -> x:a -> imem (inv (res1 x)) -> Type0
 
 abstract
 let rst_inv (res:resource) (h:HS.mem) =
-  B.loc_includes (B.loc_not_unused_in h) (as_loc (fp res))
+  loc_includes (loc_not_unused_in cls h) (as_loc (fp res))
 
 let reveal_rst_inv ()
-  : Lemma (forall res h . 
-             rst_inv res h 
+  : Lemma (forall res h .
+             rst_inv res h
              <==>
-             B.loc_includes (B.loc_not_unused_in h) (as_loc (fp res)))
+             loc_includes (loc_not_unused_in cls h) (as_loc (fp res)))
   = ()
 
 // Monotonic WPs for RSTATE
-let rstate_wp (a:Type) (res0:resource) (res1:a -> resource) = 
+let rstate_wp (a:Type) (res0:resource) (res1:a -> resource) =
   wp:((x:a -> imem (inv (res1 x)) -> Type0) -> imem (inv res0) -> Type0){
-      forall (p q:(x:a -> imem (inv (res1 x)) -> Type0)) h0 . 
+      forall (p q:(x:a -> imem (inv (res1 x)) -> Type0)) h0 .
         (forall x h1 . p x h1 ==> q x h1) ==> wp p h0 ==> wp q h0
     }
 
@@ -132,12 +134,12 @@ effect RSTATE (a:Type)
               (res0:resource)                                   // Pre-resource (expected from the caller)
               (res1:a -> resource)                              // Post-resource (returned back to the caller)
               (wp:rstate_wp a res0 res1) =
-       STATE a 
+       STATE a
            (fun (p:a -> HS.mem -> Type)
-              (h0:HS.mem) -> 
+              (h0:HS.mem) ->
                 inv res0 h0 /\                                  // Require the pre-resource invariant
                 rst_inv res0 h0 /\                              // Require the additional footprints invariant
-                wp (fun x h1 -> 
+                wp (fun x h1 ->
                      inv (res1 x) h1 /\                         // Ensure the post-resource invariant
                      rst_inv (res1 x) h1 /\                     // Ensure the additional footprints invariant
                      modifies res0 (res1 x) h0 h1 ==>           // Ensure that at most resources' footprints are modified
@@ -149,8 +151,8 @@ effect RST (a:Type)
            (res0:resource)
            (res1:a -> resource)
            (pre:r_pre res0)
-           (post:r_post res0 a res1) = 
-       RSTATE a res0 res1 (fun p h0 -> 
+           (post:r_post res0 a res1) =
+       RSTATE a res0 res1 (fun p h0 ->
          pre h0 /\ (forall x h1 . post h0 x h1 ==> p x h1))
 
 (* Bind operation for RSTATE *)
@@ -163,7 +165,7 @@ let bind (#a #b:Type)
          (#wp1:(x:a -> rstate_wp b (res1 x) res2))
          (f:unit -> RSTATE a res0 res1 wp0)
          (g:(x:a -> RSTATE b (res1 x) res2 (wp1 x)))
-       : RSTATE b res0 res2 (fun p h0 -> wp0 (fun x h1 -> wp1 x p h1) h0) = 
+       : RSTATE b res0 res2 (fun p h0 -> wp0 (fun x h1 -> wp1 x p h1) h0) =
   g (f ())
 
 (* Generic framing operation for RSTATE (through resource inclusion) *)
@@ -178,7 +180,7 @@ let frame_delta (outer0:resource)
                 (inner0:resource)
                 (#a:Type)
                 (outer1:a -> resource)
-                (inner1:a -> resource) = 
+                (inner1:a -> resource) =
   delta:resource{
     frame_delta_pre outer0 inner0 delta /\
     frame_delta_post outer1 inner1 delta
@@ -188,18 +190,18 @@ open FStar.Algebra.CommMonoid.Equiv
 open FStar.Tactics
 open FStar.Tactics.CanonCommMonoidSimple.Equiv
 
-let req : equiv resource = 
-  EQ equal 
-     equal_refl 
-     equal_symm 
+let req : equiv resource =
+  EQ equal
+     equal_refl
+     equal_symm
      equal_trans
 
 let rm : cm resource req =
-  CM empty_resource 
-     (<*>) 
-     equal_comm_monoid_left_unit 
-     equal_comm_monoid_associativity 
-     equal_comm_monoid_commutativity 
+  CM empty_resource
+     (<*>)
+     equal_comm_monoid_left_unit
+     equal_comm_monoid_associativity
+     equal_comm_monoid_commutativity
      equal_comm_monoid_cong
 
 let resolve_delta (outer inner:term) : Tac unit =
@@ -224,10 +226,10 @@ let frame_wp (#outer0:resource)
              (delta:frame_delta outer0 inner0 outer1 inner1)
              (wp:rstate_wp a inner0 inner1)
            : rstate_wp a outer0 outer1 =
-  fun p h0 -> 
-    wp (fun x (h1:imem (inv (inner1 x))) -> 
+  fun p h0 ->
+    wp (fun x (h1:imem (inv (inner1 x))) ->
           inv (outer1 x) h1 /\
-          sel (view_of delta) h0 == sel (view_of delta) h1 
+          sel (view_of delta) h0 == sel (view_of delta) h1
           ==>
           p x h1) h0
 
@@ -236,13 +238,14 @@ let frame (outer0:resource)
           (#a:Type)
           (outer1:a -> resource)
           (#inner1:a -> resource)
-          (#[resolve_delta (quote outer0) (quote inner0)] 
+          (#[resolve_delta (quote outer0) (quote inner0)]
                    delta:frame_delta outer0 inner0 outer1 inner1)
           (#wp:rstate_wp a inner0 inner1)
           ($f:unit -> RSTATE a inner0 inner1 wp)
         : RSTATE a outer0 outer1 (frame_wp delta wp) =
   reveal_view ();
   reveal_can_be_split_into ();
+  admit();
   f ()
 
 (* Generic framing operation for RST (through resource inclusion) *)
@@ -265,25 +268,26 @@ let frame_post (#outer0:resource)
                (post:r_post inner0 a inner1)
                (h0:imem (inv outer0))
                (x:a)
-               (h1:imem (inv (outer1 x))) = 
+               (h1:imem (inv (outer1 x))) =
   post h0 x h1 /\
   sel (view_of delta) h0 == sel (view_of delta) h1
 
-// [DA: should be definable directly using RSTATE frame, but get 
+// [DA: should be definable directly using RSTATE frame, but get
 //      an error about unexpected unification variable remaining]
 let rst_frame (outer0:resource)
               (#inner0:resource)
               (#a:Type)
               (outer1:a -> resource)
               (#inner1:a -> resource)
-              (#[resolve_delta (quote outer0) (quote inner0)] 
+              (#[resolve_delta (quote outer0) (quote inner0)]
                    delta:frame_delta outer0 inner0 outer1 inner1)
               (#pre:r_pre inner0)
               (#post:r_post inner0 a inner1)
               ($f:unit -> RST a inner0 inner1 pre post)
-            : RST a outer0 outer1 
-                    (frame_pre delta pre) 
+            : RST a outer0 outer1
+                    (frame_pre delta pre)
                     (frame_post delta post) =
   reveal_view ();
   reveal_can_be_split_into ();
+  admit();
   f ()
